changed and adapted a bit to pred

hol/p4_policyScript.sml
@@ -28,302 +28,2191 @@ open pred_setLib;
 val _ = new_theory "p4_policy";
 
    
-
+(*)
 Type edges = ``:('a, ('a # 'a) ) alist``;
 Type labels = ``:('a , 'b ) alist``;
 
 val _ = Hol_datatype ` 
 bdd = bdd_ir of ('a # 'a edges # ('a,'b) labels)
 `;                                                                 
+*)
 
 
 
-(* possible types *)
-val _ = Hol_datatype ` 
-ty =  (* type *)
- | ty_bit of num (* bit-string *)
- | ty_struct of (string#ty) list (* struct *)
+ (* Predicate datatype *)
+val _ = Hol_datatype `
+  pred = Var of string
+       | True
+       | False
+       | And of pred => pred
+       | Or of pred => pred
+       | Not of pred
+       | Implies of pred => pred`;
+
+                                      
+                                        
+(* BDD types *)
+val _ = type_abbrev("edges", ``:(num , (num # num)) alist``);
+
+
+                        
+    
+val _ = Hol_datatype `
+  label = termn of pred
+        | non_termn of ( string option #  pred)`;
+
+               
+val _ = type_abbrev("labelings", ``:(num , label) alist``);
+val _ = type_abbrev("BDD", ``:num # edges # labelings``);
+
+
+
+
+
+
+val get_leaves_list_def = Define `
+  get_leaves_list (edges : edges) =
+    nub (FILTER (\x. ~(MEM x (MAP FST edges))) 
+           (FLAT (MAP (\(k, (v1, v2)). [v1; v2]) edges)))
+`;
+
+
+        
+
+    
+(* Helper functions *)
+val getLeaves_def = Define `
+   getLeaves [] r = [r] ∧
+   getLeaves edges r = get_leaves_list (edges)
+`;
+
+
+
+
+Definition edges_acyclic_def:
+  edges_acyclic (edges:edges) =
+  let nl = MAP (\(n,n',n''). (n,n')) edges;
+      nr = MAP (\(n,n',n''). (n,n'')) edges
+  in
+     acyclic(LIST_TO_SET(nl) ∪ LIST_TO_SET(nr) )
+End
+
+
+
+
+val is_lookup_defined_def = Define `
+    is_lookup_defined l1 n =
+     ? y . ALOOKUP l1 n = SOME y 
 `;
         
-Type descriptor = ``:(string#ty) list``;
+val is_lookup_non_leaf_def = Define `
+    is_lookup_non_leaf l1 n =
+     ? x p . ALOOKUP l1 n = SOME (non_termn (SOME x, p))
+`;
 
-Type field = ``:string``;
+val is_lookup_leaf_def = Define `
+    is_lookup_leaf l1 n =
+     ? p . ALOOKUP l1 n = SOME (non_termn (NONE, p))
+`;
+        
+
+
+
+
+
+        
+Definition BDD_WF_def:
+  BDD_WF ((r,edges,labels):BDD) =
+  (ALL_DISTINCT (MAP FST edges)  ∧ ALL_DISTINCT (MAP FST labels)  ∧
+    (∀ n . is_lookup_defined edges n ⇔ is_lookup_non_leaf labels n ) ∧
+    (∀ n . ALOOKUP edges n = NONE  ⇔   (is_lookup_leaf labels n
+                                        ∨ ALOOKUP labels n= SOME (termn True)
+                                        ∨ ALOOKUP labels n= SOME (termn False))
+    ))
+End
+
+
+
+
+Type ord = ``:(string -> string -> bool )``
+        
+
+Definition WF_o_def:
+(WF_o order) =    (( !(x:ord).   (order x x) ) /\
+  		 ( !x y.   order x y  ==> ~order y x ) /\
+                 ( !x y z. order x y /\ order y z  ==> order x z ))
+End
+
+        
+Definition ordered_el_def:
+ordered_el (order:ord) el1 el2  =
+   order el1 el2
+End
+
+        
+Definition ordered_list_def:
+ordered_list (order:ord) l  =
+    ! i . i < LENGTH l - 2  ==> order (EL i l) (EL (SUC i) l)
+End
+
+
+
+Definition find_index_x_def:        
+find_index_x xl x =
+INDEX_OF
+End
+        
+
+Definition BDD_ordered_def:
+BDD_ordered ((r,edges,labels):BDD) xl =
+∀ n n' n'' x x' x'' p p' p'' i i' i''.
+  ALOOKUP edges n = SOME (n',n'') ⇒
+  ((ALOOKUP labels n   =  SOME (non_termn(SOME x,   p   )) ∧
+    ALOOKUP labels n'  =  SOME (non_termn(SOME x',  p'  )) ∧
+    INDEX_OF x xl  = SOME i ∧
+    INDEX_OF x' xl = SOME i' 
+    ⇒ 
+    i' < i 
+   )
+   ∧
+   (ALOOKUP labels n   =  SOME (non_termn(SOME x,   p   )) ∧
+    ALOOKUP labels n'' =  SOME (non_termn(SOME x'', p'' )) ∧
+    INDEX_OF  x   xl = SOME i ∧
+    INDEX_OF  x'' xl = SOME i''
+    ⇒ 
+    i'' < i
+   )
+  )
+End
+        
+
+        
+    
+
+                                        
+(* Predicate semantics *)
+val Sem_rule_def = Define `
+  (Sem_rule (Var x) m_v = (ALOOKUP m_v x) ) /\
+  (Sem_rule True _ = SOME T) /\
+  (Sem_rule False _ = SOME F) /\
+  (Sem_rule (And p q) m_v = 
+    case (Sem_rule p m_v, Sem_rule q m_v)  of
+    | (SOME b, SOME b') => SOME (b ∧ b')
+    | (_,_) => NONE
+    ) /\
+  (Sem_rule (Or p q) m_v = 
+    case (Sem_rule p m_v, Sem_rule q m_v)  of
+    | (SOME b,SOME b') => SOME (b ∨ b')
+    | (_,_) => NONE
+    ) /\
+    (Sem_rule (Not p) m_v = 
+    case (Sem_rule p m_v)  of
+    | SOME b => SOME (~b)
+    | _ => NONE
+    ) /\
+    (Sem_rule (Implies p q) m_v = 
+    case (Sem_rule p m_v, Sem_rule q m_v)  of
+    | (SOME b,SOME b') => SOME (b ⇒ b')
+    | (_,_) => NONE
+    ) `;
+
+
+
+
+                                        
+(* Predicate semantics *)
+Definition apply_Sem_rule_def:
+(apply_Sem_rule (NONE) m_v = NONE ) /\
+(apply_Sem_rule (SOME p) m_v = Sem_rule p m_v ) 
+End
+
+
+
+        
+(*                                                                        
+EVAL “Sem_rule (Or (Var "a") (Var "b")) [("a",T);("b",F)]”
+EVAL “Sem_rule (And (Var "b") (Var "b")) [("a",F);("b",F)]”
+EVAL “Sem_rule (Or (Var "b") ((Implies (Var "a") (Var "b")))) [("a",F);("b",F)]”
+EVAL “Sem_rule (Or (Var "a") False) []”
+
+*)
+
+
+                                                                        
+   
+
+(* P[x -> T] *)     
+Definition mk_substitute_pred_def:
+  (mk_substitute_pred (True) (Var x) b = True) ∧
+  (mk_substitute_pred (False) (Var x) b = False) ∧
+  (mk_substitute_pred (Var (x')) (Var x) b = if (x=x') then b else (Var x') ) ∧
+  (mk_substitute_pred (And c c' ) (Var x) b =
+      (And (mk_substitute_pred c (Var x) b) (mk_substitute_pred c' (Var x) b ))) ∧
+  (mk_substitute_pred (Or c c') (Var x) b =
+      (Or (mk_substitute_pred c (Var x) b) (mk_substitute_pred c' (Var x) b ))) ∧
+  (mk_substitute_pred (Not c) (Var x) b=
+      (Not (mk_substitute_pred c (Var x) b)))
+End
+
+
+(*        
+EVAL “mk_substitute_pred (Or (Var "a") (Var "b")) "b" True”
+EVAL “mk_substitute_pred (Or (Var "b") (Var "b")) "b" True”
+EVAL “mk_substitute_pred (Or (Var "b") ((Or (Var "a") (Var "b")))) "b" True”
+*)
+
+
+
+Definition is_termn_def:
+  is_termn (l:label) =
+  case l of
+  | termn _ => T
+  | non_termn _ => F
+End
+
+
+Definition extract_nontermn_def:
+  extract_nontermn [] = SOME [] ∧
+  extract_nontermn ((n,l)::leaves_labels) =
+  case (extract_nontermn leaves_labels) of
+  | SOME l' => (
+    case (l) of
+    | termn p  => SOME l'
+    | non_termn (NONE , p) => SOME ((n ,p)::l')
+    | non_termn (SOME x,p) => NONE
+    ) 
+  | NONE => NONE
+End
+
+(*        
+EVAL “extract_nontermn [(1,termn True); (2, termn False); (3,  non_termn (SOME "a",(And (Var "a") (Var "b"))) )] ”;
+EVAL “extract_nontermn [(1,termn True); (2, termn False); (3,  non_termn (NONE,(And (Var "a") (Var "b"))) )] ”;
+*)
+
+
 
 
      
-val _ = Hol_datatype ` 
-h =
-| h_f of field
-| h_acc of (field list)
-| h_slice of (field list) => num => num`;
+        
+Definition extract_termn_def:
+  extract_termn [] = SOME [] ∧
+  extract_termn ((n,l)::leaves_labels) =
+  case (extract_termn leaves_labels) of
+  | SOME l' => (
+    case (l) of
+    | termn True  => SOME ((n , termn True)::l')
+    | termn False  => SOME ((n ,termn False)::l')
+    | termn _  => NONE
+    | non_termn _ => SOME l'
+    ) 
+  | NONE => NONE
+End
+
+
+(*        
+EVAL “extract_termn [(1,termn True); (2, termn False); (3,  non_termn (SOME "a",(And (Var "a") (Var "b"))) );
+                     (2, termn False)] ”;
+EVAL “extract_termn [(1,termn True); (2, termn False); (3,  termn (And True True))] ”;
+*)
+       
+
+Definition getLabels_def:
+  (getLabels labels [] = SOME [] ) ∧
+  (getLabels labels (n::leaves) =
+   case (getLabels labels leaves) of
+   | SOME l =>
+       (
+       case (ALOOKUP labels n) of
+       | NONE => NONE
+       | SOME lbl => SOME ((n,lbl)::l)
+       )
+   | NONE => NONE
+  )
+End
+       
+        
+Definition leaves_pred_sub_def:
+  leaves_pred_sub (nodes_labels:(num#pred)list) x =
+  MAP
+  (\(n,p).(n,x,mk_substitute_pred p (Var x) True,mk_substitute_pred p (Var x) False)) nodes_labels 
+End
+
+        
+
+Definition mk_new_labels_def:
+  mk_new_labels [] (c:num) =  [] ∧
+  mk_new_labels ((n,x',(label,label'))::rest) c =  (c, label)::(c+1, label')::(mk_new_labels rest (c+2)) 
+End
+
+        
+
+Definition mk_new_edges_def:
+  mk_new_edges []                c =  [] ∧
+  mk_new_edges ((n:num,x',(p,p'))::rest) (c:num) =  (n, c, c+1)::(mk_new_edges rest (c+2))     
+End
 
 
 
-val _ = Hol_datatype ` 
-aop = 
- | aop_le (* less or equal *)
- | aop_ge (* greater or equal *)
- | aop_lt (* less *)
- | aop_gt (* greater *)
- | aop_neq (* not equal *)
- | aop_eq (* equal *)
- | aop_and (* bitwise and *)
- | aop_xor (* bitwise xor *)
- | aop_or (* bitwise or *)
-`;
+
+        
+Definition simp_pred_def:
+  (simp_pred (Var x) = Var x) /\
+  (simp_pred True = True) /\
+  (simp_pred False = False) /\
+  (simp_pred (And p q) =
+    let p' = simp_pred p in
+    let q' = simp_pred q in
+      case (p', q') of
+      |  (True, True) => True
+      | (False,  _) => False
+      | (_, False) => False
+      | (True, q') => q'
+      | (p', True) => p'
+      | _ => And p' q') /\
+  (simp_pred (Or p q) =
+    let p' = simp_pred p in
+    let q' = simp_pred q in
+      case (p', q') of
+      |  (False, False) => False
+      | (False, q') => q'
+      | (p', False) => p'
+      | (True, _) => True
+      | (_, True) => True
+      | _ => Or p' q') /\
+  (simp_pred (Not p) =
+    let p' = simp_pred p in
+      case p' of
+      |  True => False
+      | False => True
+      | _ => Not p') /\
+  (simp_pred (Implies p q) =
+    let p' = simp_pred p in
+    let q' = simp_pred q in
+      case (p', q') of
+      |  (True, False) => False
+      | (False, _) => True
+      | (True, q') => q'
+      | _ => Implies p' q')
+End
+
+
+Definition simp_pred_list_def:
+  simp_pred_list leaves_sub =
+  MAP (\(n,x,p,p'). (n,x,simp_pred p , simp_pred p')) leaves_sub
+End
+
+
+        
    
-(*binop as we have in P4 semantics*)
-val _ = Hol_datatype ` 
-exp =
-exp_aop of h => aop => num  `; (*arithmetic expressions*)
+Definition determine_termn_def:
+  determine_termn (p:pred) =
+  case p of
+  | True => termn True
+  | False => termn False
+  | _ => non_termn (NONE,p) 
+End
+
+Definition determine_termn_list_def:
+  determine_termn_list nodes_simp =
+   MAP (\(n,x,p,p'). (n, x, determine_termn p , determine_termn p' )) nodes_simp
+End
+        
+          
 
 
 
-(*type of conditions is generic so the proofs are applied to both semantics of rules and also the BDD translation*)        
-val _ = Hol_datatype ` 
-c =
-c_b of bool 
-|c_e of 'a  (* for the BDD this is a string, for the rules semantics it is exp ?*)     
-|c_and of c => c
-|c_or of c => c
-|c_neg of c
-`;  
 
-Type rule = ``:('a c # string)``;
+        
+
+Definition mk_distict_labels_def:
+  (mk_distict_labels [] l'= []) ∧
+  (mk_distict_labels ((p,n)::l) l' =
+   case (ALOOKUP l' p) of
+   | SOME n' => mk_distict_labels l l'
+   | NONE => (p,n)::(mk_distict_labels l ((p,n)::l') )
+  )          
+End
+
+
+(*
+EVAL “mk_distict_labels [("a",1);("b",2)] [] ”
+EVAL “mk_distict_labels [("a",1);("a",2)] [] ”
+EVAL “mk_distict_labels [("a",1);("a",2);("b",1);("a",3)] [] ”
+EVAL  “mk_distict_labels [("p",1);("c",2)] []”
+*)
+        
+
+        
+Definition replace_mem_def:
+(replace_mem [] m = []) ∧
+(replace_mem ((p,n)::l) (p',n') =
+ if p'=p then
+   (p,n')::replace_mem l (p',n')
+ else
+   (p,n)::replace_mem l (p',n')    
+)    
+End
+
+
+
+Definition replace_all_def:
+  (replace_all l [] = l) ∧
+  (replace_all l (h::disctict_l) =
+    let replaced = replace_mem l h in
+         replace_all replaced disctict_l
+  )     
+End
+
+ 
+
+Definition merge_leaves_labels_def:
+  (merge_leaves_labels [] = []) ∧
+  (merge_leaves_labels l =
+    let distinct_l = mk_distict_labels l [] in           
+      replace_all l distinct_l
+  )     
+End
+        
+(*        
+EVAL “merge_leaves_labels [("p",1);("c",2);("p",1)]”;
+EVAL “merge_leaves_labels [("p",1);("p",2);("p",1)]”;
+*)
+        
+
+
+Definition mirror_domain_range_def:
+  mirror_domain_range l =
+    MAP (\(x,y). (y,x)) l
+End
+
+
+
+
+Definition update_merged_edges_def:
+  (update_merged_edges [] [] = [])  ∧
+  (update_merged_edges ((n1,p)::(n1',p')::new_labels) ((n2,n2',n2'')::new_edges) =
+     ((n2,n1,n1')::update_merged_edges new_labels new_edges))
+End        
+
+
+Definition segment_non_term_def:           
+  segment_non_term leaves_termn labelings =
+  if leaves_termn = [] then
+     labelings
+  else
+    SEG (LENGTH leaves_termn) 0 labelings
+End          
+
+Definition merge_all_nodes_def:
+  merge_all_nodes leaves_termn (new_edges:edges) (new_labels:labelings) =
+              
+  (* first we merge all nodes that are newly created within the same level, aka new leaves*)
+  let mirrored_labeling = mirror_domain_range (leaves_termn++new_labels) in
+       let merged_leaves = merge_leaves_labels mirrored_labeling in
+         let mirrored_labeling = mirror_domain_range merged_leaves in
+             
+           let new_labels' =  segment_non_term leaves_termn mirrored_labeling in
+             let new_edges'  =  update_merged_edges new_labels' new_edges in
+               (new_edges',nub new_labels')
+End
+
+         
+
+Definition update_non_term_var_def:        
+  update_non_term_var leaves_nontermn x =
+  MAP (\(n,p). (n, non_termn (SOME x,p))) leaves_nontermn
+End
+
+
+
+
+Definition non_term_leaf_updt_def:
+  non_term_leaf_updt (l1:(num # label) list) (x:string) =
+    MAP (λ(n, lbl).
+      case lbl of
+      | termn p => (n, termn p)
+      | non_termn (NONE, p) => (n, non_termn (SOME x, p))
+      | non_termn (SOME x', p) => (n, non_termn (SOME x', p))
+        ) l1
+End
+
+
+
+Definition body_of_mk_def:
+  body_of_mk (BDD:BDD) (x:string) (c:num) =
+  (let (r,edges,labels) = BDD in
+    (let leaves = getLeaves edges r in
+       (case (getLabels labels leaves) of
+        | SOME leaves_labels =>
+            ( case (extract_termn leaves_labels) of
+              (* this is incorrect , there can be non terminat *)
+              | SOME leaves_termn =>
+                  ( case (extract_nontermn leaves_labels) of
+                    | SOME leaves_nontermn =>
+                        ( let leaves_sub = leaves_pred_sub leaves_nontermn x in
+                            let simp_leaves = simp_pred_list leaves_sub in
+                              let simp_leaves' = determine_termn_list simp_leaves in
+                                let new_labels = mk_new_labels simp_leaves' c in
+                                  let new_edges = mk_new_edges simp_leaves' c in
+                                    let label_leaf_updated = non_term_leaf_updt labels x
+                                    in
+                                     SOME (((r,  edges ++ new_edges, label_leaf_updated++new_labels):BDD),  (c + LENGTH leaves_nontermn + 1))             
+                        )
+                    | NONE => NONE
+                  )
+              | NONE => NONE
+           )
+        | NONE => NONE
+       )
+   ))
+End
+
+
+Definition mk_BDDPred_def:
+  (mk_BDDPred (BDD:BDD) l [] c = SOME BDD) ∧
+  (mk_BDDPred (BDD:BDD) l (x::xs) c =
+   case (body_of_mk BDD (x:string) (c:num)) of
+   | SOME (BDD',c') => mk_BDDPred BDD' (x::l) xs c'
+   | NONE => NONE 
+  )
+End
+
+
+
+        
+
+(*
+EVAL “mk_BDDPred (0,[],[(0, non_termn (NONE, (Var "a")))]) [] ["a"] 1”;
+EVAL “mk_BDDPred (0,[],[(0, non_termn (SOME "a", (Var "a")))]) [] ["a"] 1”;
+EVAL “mk_BDDPred (0,[],[(0, non_termn (NONE, (And (Var "a") (Var "b"))))]) [] ["a";"b"] 1”;
+EVAL “mk_BDDPred (0,[],[(0, non_termn (NONE, Or (Var "a") (Var "b")))]) [] ["a";"b";"c"] 1”;
+*)                
+
+
+                                                                                
+(*
+val toBDD_pred_def = Define `
+  toBDD_pred P vars = mk_BDDPred (0, [], [(0, non_termn ( HD vars , P))]) vars 1`;
+*)
+
+
+
+Definition size_of_tree_def:
+  size_of_tree (edges:edges) (n:num) =
+               
+( case ALOOKUP edges n of
+  | SOME (l,r) => 1 + size_of_tree (DELETE_ELEMENT (n,l,r) edges) l + size_of_tree (DELETE_ELEMENT (n,l,r) edges) r
+  | NONE =>  (1:num)
+)
+Termination
+WF_REL_TAC `measure (\(edges,n). LENGTH edges)` >>
+REPEAT STRIP_TAC >>
+gvs[LENGTH_DELETE_ELEMENT_LE, ALOOKUP_MEM]
+End
+
+                                                       
+        
+
+Definition from_pred_to_bool_def:
+  from_pred_to_bool p mv =
+  case p of
+  |  (termn True)  => SOME T
+  |  (termn False) => SOME F
+  |  (termn _) => NONE
+  |  (non_termn (_,p)) => Sem_rule p mv
+End
+
+
+
+        
+(*
+Definition Sem_BDDpred_fun_def:
+  Sem_BDDpred_fun ((root,edges,labels):BDD) (m_v:(string#bool)list) n=
+    case ALOOKUP edges n of
+      | NONE =>
+          (case ALOOKUP labels n of
+             | SOME (termn True)  => SOME T
+             | SOME (termn False) => SOME F
+             | SOME (termn _) => NONE
+             | SOME (non_termn (_,p)) => Sem_rule p m_v
+             | NONE => NONE )
+      | SOME (l,r) =>
+          case ALOOKUP labels n of
+             | SOME (non_termn (SOME x,p)) =>
+                   ( case ALOOKUP m_v x of
+                        | SOME T => Sem_BDDpred_fun (root,edges,labels) m_v r
+                        | SOME F => Sem_BDDpred_fun (root,edges,labels) m_v l
+                        | NONE => NONE )
+             | _ => NONE
+End
+*)
+
+        
+
+Inductive BDD_pred_sem:
+(* defn pred_red *)
+  
+[pred_red_leaf:]
+  ( ∀ (root:num) (edges:edges) (labels:labelings) (mv:(string#bool)list) (n:num) (p:label).
+      ALOOKUP edges n = NONE ∧
+      ALOOKUP labels n  = SOME p 
+      ⇒      
+      BDD_pred_sem (r,edges,labels) mv n (from_pred_to_bool p mv) 
+  )
+  
+  
+[pred_red_internal_T:]
+  ( ∀ (root:num) (edges:edges) (labels:labelings) (mv:(string#bool)list) (n:num) (l:num) (r:num) (pred:pred) (x:string) (b':bool option).
+      ALOOKUP edges n = SOME (l,r) ∧
+      ALOOKUP labels n  = SOME (non_termn (SOME x ,pred)) ∧
+      ALOOKUP mv x = SOME T ∧
+      BDD_pred_sem (root,edges,labels) mv l b'
+      ⇒      
+      BDD_pred_sem (root,edges,labels) mv n b'
+  )
+  
+[pred_red_internal_F:]
+  ( ∀ (root:num) (edges:edges) (labels:labelings) (mv:(string#bool)list) (n:num) (l:num) (r:num) (pred:pred) (x:string) (b':bool option).
+      ALOOKUP edges n = SOME (l,r) ∧
+      ALOOKUP labels n  = SOME (non_termn (SOME x ,pred)) ∧
+      ALOOKUP mv x = SOME F ∧
+      BDD_pred_sem (root,edges,labels) mv r b'
+      ⇒      
+      BDD_pred_sem (root,edges,labels) mv n b'
+  )            
+End
+
+
+       
+
+       
+Definition get_prop_def:
+  get_prop labels n =
+  (case ALOOKUP labels n of
+   | SOME (termn True) => SOME True
+   | SOME (termn False) => SOME False
+   | SOME (termn _) => NONE
+   | SOME (non_termn (x,p)) => SOME p
+   | NONE => NONE
+  )
+End
+
+
+               
+(* correct sem definition *)
+
+Definition correct_sem_def:
+  correct_sem (BDD:BDD)  =
+  ∀ n mv b r edges labels.
+      BDD = (r,edges,labels) ∧
+      BDD_pred_sem BDD mv n b ⇒
+       b = apply_Sem_rule (get_prop labels n) mv         
+End 
+
+
+Definition FV_def:
+  FV (Var x) = [x] ∧
+  FV True = [] ∧
+  FV False = [] ∧
+  FV (And p q) = nub (FV p ++ FV q) ∧
+  FV (Or p q) = nub (FV p ++ FV q) ∧
+  FV (Not p) = FV p ∧
+  FV (Implies p q) = nub (FV p ++ FV q)
+End
+
+
+
+
+Theorem simp_pred_imp_mem:          
+∀ p x .
+simp_pred p = Var x ⇒
+MEM x (FV p)
+Proof
+    Induct >>
+rw[simp_pred_def, FV_def] >> gvs[AllCaseEqs()]
+QED
+
+
+Theorem mem_imp_sem_rule:        
+  ∀p mv. (∀x. MEM x (FV p) ⇒ (∃b. ALOOKUP mv x = SOME b)) ⇒
+     Sem_rule p mv ≠ NONE ∧ ∃ b' . Sem_rule p mv = SOME b'
+Proof
+  Induct >>
+  rw[simp_pred_def, FV_def] >> gvs[AllCaseEqs()] >>
+  gvs[Sem_rule_def, simp_pred_def] >>
+  REPEAT (BasicProvers.FULL_CASE_TAC >> gvs[]) 
+QED
+
+
+
+
+
+        
+
+(* must add free variables condition here,
+   Otherwise we might need to prove something like this which is incorrect:
+   Sem_rule (And True (Var x)) mv = Sem_rule (simp_pred (And True (Var x))) mv
+   where the simplification will give us true, even if Var x is not in mv = NONE
+
+   EDIT: there are many thing that can go wrong, actuallt false and none
+*)       
+          
+
+
+Theorem simplification_correct:
+  ∀p mv. (∀x. MEM x (FV p) ⇒ (∃b. ALOOKUP mv x = SOME b)) ⇒
+     Sem_rule p mv = Sem_rule (simp_pred p) mv
+Proof
+  Induct_on `p` >-
+   (rw[simp_pred_def, Sem_rule_def]) >-
+   (rw[simp_pred_def, Sem_rule_def]) >-
+   (rw[simp_pred_def, Sem_rule_def]) >>
+
+  rpt strip_tac >>
+  IMP_RES_TAC mem_imp_sem_rule >>
+
+  LAST_X_ASSUM (STRIP_ASSUME_TAC o (Q.SPECL [‘mv’])) >>
+  gvs[FV_def] >>
+  gvs[Sem_rule_def] >>   
+
+  rw[Sem_rule_def, simp_pred_def] >>   
+  REPEAT (BasicProvers.FULL_CASE_TAC >> gvs[]) >>
+  gvs[Sem_rule_def, simp_pred_def] >>
+  
+  FIRST_X_ASSUM (STRIP_ASSUME_TAC o (Q.SPECL [‘s’])) >>
+  IMP_RES_TAC simp_pred_imp_mem >>
+  gvs[]
+        
+QED
+
+        
+             
+
+
+
+    
+
+    
+Theorem non_term_leaf_updt_concat:    
+∀ x l1 l2.
+non_term_leaf_updt (l1++l2) x = non_term_leaf_updt l1 x ++ non_term_leaf_updt l2 x
+Proof    
+fs[non_term_leaf_updt_def]
+QED
+
+
+Theorem non_term_leaf_updt_cons:        
+∀ l h x . non_term_leaf_updt (h::l) x = non_term_leaf_updt [h] x ++ non_term_leaf_updt l x
+Proof
+fs[non_term_leaf_updt_def]
+QED
+
+
+
+        
+        
+Theorem non_term_leaf_updt_rec:
+∀ l x x'.                                                                                
+non_term_leaf_updt ( non_term_leaf_updt l x ) x' =  non_term_leaf_updt l x 
+Proof
+  Induct >>
+  rpt strip_tac >-
+   gvs[non_term_leaf_updt_def] >>
+
+   Cases_on ‘h’ >>
+   Cases_on ‘r’ >>
+   gvs[non_term_leaf_updt_def] >>
+
+   Cases_on ‘p’ >>
+   Cases_on ‘q'’ >>
+   gvs[non_term_leaf_updt_def]
+QED
+   
+
+
+
+                                                                  
+Theorem mk_BDDPred_output:
+  ∀ vars vars_consumed r r' edges edges' labels labels'  c.
+    vars ≠ [] ∧ 
+mk_BDDPred (r, edges, labels) vars_consumed vars c = SOME (r', edges', labels') ⇒
+ r = r' ∧ ∃ edges'' labels''. edges' = edges ++ edges'' ∧ labels' = (non_term_leaf_updt labels (HD vars)) ++ labels''
+Proof                                                                                                                                                         
+Induct_on ‘vars’ >- fs[mk_BDDPred_def] >>
+
+Cases_on ‘vars = []’ >> gvs[] >>
+rpt strip_tac >>
+gvs[mk_BDDPred_def, body_of_mk_def] >> 
+REPEAT (BasicProvers.FULL_CASE_TAC >> gvs[]) >>
+
+‘∃ leaves_sub . leaves_pred_sub x' h = leaves_sub’ by gvs[] >>
+‘∃ simp_leaves . simp_pred_list leaves_sub = simp_leaves’ by gvs[] >>
+‘∃ simp_leaves' . determine_termn_list simp_leaves = simp_leaves'’ by gvs[] >>
+    
+rgs[] >>
+(RES_TAC) >>
+
+gvs[non_term_leaf_updt_rec, non_term_leaf_updt_concat]
+QED                           
+
+
+
+
+                     
+             
+
+Theorem SNOC_rw:
+∀ l x .
+SNOC x l = l ++[x]
+Proof
+gvs[SNOC]
+QED
+
+
+        
+Definition get_string_in_label_def:
+  get_string_in_label (labels:labelings)  vars_consumed n =
+  case ALOOKUP (labels:labelings) n of
+  | NONE =>  0
+  | SOME lbl => (
+    case lbl of
+    | termn p =>  0
+    | non_termn (NONE,p) =>  0
+    | non_termn (SOME x,p) =>  THE (INDEX_OF x vars_consumed) 
+    ) 
+End
+
+
+
+val move_forall_fst_tac : tactic =
+  FIRST_X_ASSUM (fn th =>
+  let val (vars, body) = strip_forall (concl th) in
+    if null vars then
+      NO_TAC
+    else
+      let val new_vars = tl vars @ [hd vars]
+          val th_body = SPEC_ALL th
+          val new_th = GENL new_vars th_body
+      in
+      POP_ASSUM (K ALL_TAC) >> ASSUME_TAC new_th
+       end
+   end
+);
+
+
+
+
+   
+                  
+(*
+  measureInduct_on `get_string_in_label labels  vars_consumed n` >>
+*)                   
+
+
+
+(*
+Inductive BDD_ind:
+(* defn pred_red *)
+  
+[BDD_ind_leaf:]
+  ( ∀ (root:num) (edges:edges) (labels:labelings) (n:num) (P:(BDD -> 'a)).
+      ALOOKUP edges n = NONE ∧
+      ALOOKUP labels n  = SOME p 
+      ⇒      
+      BDD_ind (r,edges,labels) n (P (r,edges,labels)) 
+  )
+  
+  
+[BDD_ind_internal_T:]
+  ( ∀ (root:num) (edges:edges) (labels:labelings) (n:num) (l:num) (r:num) (pred:pred) (x:string) (a:'a).
+      ALOOKUP edges n = SOME (l,r) ∧
+      ALOOKUP labels n  = SOME (non_termn (SOME x ,pred)) ∧
+      BDD_ind (root,edges,labels) l a
+      ⇒      
+      BDD_ind (root,edges,labels) n a
+  )
+  
+[BDD_ind_internal_F:]
+  ( ∀ (root:num) (edges:edges) (labels:labelings) (n:num) (l:num) (r:num) (pred:pred) (x:string) (a:'a).
+      ALOOKUP edges n = SOME (l,r) ∧
+      ALOOKUP labels n  = SOME (non_termn (SOME x ,pred)) ∧
+      BDD_ind (root,edges,labels) r a
+      ⇒      
+      BDD_ind (root,edges,labels) n a
+  )           
+End
+*)
+
+
+
+(*
+Definition correct_sem_def:
+  correct_sem (BDD:BDD)  =
+  ∀ n mv b r edges labels.
+      BDD = (r,edges,labels) ∧
+      BDD_pred_sem BDD mv n b  ⇒
+       b = apply_Sem_rule (get_prop labels n) mv         
+End  
+*)
+
+
+
+          
+Theorem BDD_pred_sem_determ:
+  ∀ n BDD mv b b'.        
+  BDD_pred_sem BDD mv n b ∧
+  BDD_pred_sem BDD mv n b' ⇒
+  (b=b')
+Proof
+ Induct_on ‘BDD_pred_sem’ >>        
+ rpt strip_tac >>
+ rgs[Once BDD_pred_sem_cases]
+QED
+
+
+Definition mv_dom_bdd_def:
+  mv_dom_bdd mv (root,edges,labels) = 
+  ∀ n pred x.
+    (ALOOKUP labels n = SOME (non_termn (SOME x,pred))) ⇔
+    is_lookup_defined mv x
+End
+
+
+Definition consumed_dom_bdd_def:
+  consumed_dom_bdd vars_consumed ((root,edges,labels):BDD) = 
+  ∀ n pred x.
+    (ALOOKUP labels n = SOME (non_termn (SOME x,pred))) ⇔
+    MEM x vars_consumed
+End        
+
+
+Theorem MEM_INDEX_OF:           
+∀ l x .
+MEM x l ⇒
+∃ i . INDEX_OF x l = SOME i
+Proof                                
+Induct >>                                
+rpt strip_tac >>
+gvs[INDEX_OF_def,  INDEX_FIND_def] >>
+Cases_on ‘x=h’ >> gvs[] >>
+RES_TAC >>
+PairCases_on ‘z’ >>
+imp_res_tac P_implies_next >>
+gvs[]
+QED
+          
+
+Theorem BDD_pred_sem_exsists_inter:
+∀ vars_consumed x' labels root edges mv n n1 n2 pred b.            
+  BDD_ordered (root,edges,labels) vars_consumed ∧
+  mv_dom_bdd mv (root,edges,labels)  ∧
+  consumed_dom_bdd vars_consumed (root,edges,labels) ∧
+  BDD_WF (root,edges,labels) ∧
+  ALOOKUP edges n = SOME (n1,n2) ∧
+  ALOOKUP labels n = SOME (non_termn (SOME x',pred)) ∧
+  ALOOKUP mv x' = SOME b 
+⇒
+∃b'. ALOOKUP mv x' = SOME T ∧ BDD_pred_sem (root,edges,labels) mv n1 b' ∨
+    ALOOKUP mv x' = SOME F ∧ BDD_pred_sem (root,edges,labels) mv n2 b'
+Proof
+  ntac 2 strip_tac >>
+  measureInduct_on `THE(INDEX_OF x' vars_consumed)` >>
+  rpt strip_tac >>
+  Cases_on ‘b’ >> gvs[] >|[
+    
+    simp[Once BDD_pred_sem_cases] >>
+    rgs[] >>
+    Cases_on ‘ALOOKUP edges n1’ >> gvs[] >|[
+      gvs[BDD_WF_def, is_lookup_leaf_def]
+      ,
+      
+      PairCases_on ‘x’ >> gvs[] >>
+     
+      subgoal ‘∃pred x'.ALOOKUP labels n1 = SOME (non_termn (SOME x',pred))’ >-
+       (
+       rgs[Once BDD_WF_def, Once is_lookup_non_leaf_def, Once is_lookup_defined_def] >>
+       first_x_assum (strip_assume_tac o (Q.SPECL [‘n1’])) >>
+       gvs[]
+       ) >>
+      gvs[] >>
+      
+      subgoal ‘∃b . ALOOKUP mv x'' = SOME b’ >-
+       (
+       gvs[mv_dom_bdd_def, is_lookup_defined_def]
+       ) >>
+      
+      ‘MEM x' vars_consumed ∧ MEM x'' vars_consumed’ by rgs[Once consumed_dom_bdd_def] >>
+      imp_res_tac MEM_INDEX_OF >>
+      
+      subgoal ‘THE (INDEX_OF x'' vars_consumed) < THE (INDEX_OF x' vars_consumed)’ >-
+       (
+       
+       rgs[Once BDD_ordered_def]>>
+       first_x_assum (strip_assume_tac o (Q.SPECL [‘n’,‘n1’, ‘n2’,‘x'’, ‘x''’,‘x'''’,
+                                                   ‘pred’, ‘pred'’,‘pred'''’,‘i'’,‘i’,‘i''’])) >>
+       
+       rgs[]
+       ) >>
+      
+      first_x_assum (strip_assume_tac o (Q.SPECL [‘INDEX_OF (x'':string) (vars_consumed: string list)’])) >>
+      gvs[] >>
+      first_x_assum (strip_assume_tac o (Q.SPECL [‘x''’, ‘vars_consumed’])) >>
+      gvs[] >>
+      METIS_TAC[]
+    ]
+    ,
+    
+    simp[Once BDD_pred_sem_cases] >>
+    rgs[] >>
+    Cases_on ‘ALOOKUP edges n2’ >> gvs[] >|[
+        gvs[BDD_WF_def, is_lookup_leaf_def]
+        ,
+        
+        PairCases_on ‘x’ >> gvs[] >>
+
+        subgoal ‘∃pred x'.ALOOKUP labels n2 = SOME (non_termn (SOME x',pred))’ >-
+         (
+         rgs[Once BDD_WF_def, Once is_lookup_non_leaf_def, Once is_lookup_defined_def] >>
+         first_x_assum (strip_assume_tac o (Q.SPECL [‘n2’])) >>
+         gvs[]
+         ) >>
+        gvs[] >>
+        
+
+        subgoal ‘∃b . ALOOKUP mv x'' = SOME b’ >-
+         (
+         gvs[mv_dom_bdd_def, is_lookup_defined_def]
+         ) >>
+        
+        
+        ‘MEM x' vars_consumed ∧ MEM x'' vars_consumed’ by rgs[Once consumed_dom_bdd_def] >>
+        imp_res_tac MEM_INDEX_OF >>
+       
+        
+        subgoal ‘THE (INDEX_OF x'' vars_consumed) < THE (INDEX_OF x' vars_consumed)’ >-
+         (
+         
+         rgs[Once BDD_ordered_def]>>
+         first_x_assum (strip_assume_tac o (Q.SPECL [‘n’,‘n1’, ‘n2’,‘x'’, ‘x'''’,‘x''’,
+                                                     ‘pred’, ‘pred'''’,‘pred'’,
+                                                     ‘i'’,‘i''’,‘i’])) >>
+         
+         rgs[]
+         ) >>
+        
+        first_x_assum (strip_assume_tac o (Q.SPECL [‘INDEX_OF (x'':string) (vars_consumed: string list)’])) >>
+        gvs[] >>
+        first_x_assum (strip_assume_tac o (Q.SPECL [‘x''’, ‘vars_consumed’])) >>
+        gvs[] >>
+        METIS_TAC[]
+      ]
+                                           
+    ]          
+QED
+
+
+
+        
+Theorem BDD_pred_sem_exsists:
+  ∀ BDD mv n vars_consumed.
+    BDD_ordered BDD vars_consumed ∧
+    mv_dom_bdd mv BDD  ∧
+    consumed_dom_bdd vars_consumed BDD ∧
+    BDD_WF BDD ⇒
+  ∃ b . BDD_pred_sem BDD mv n b
+Proof
+ rgs[Once BDD_pred_sem_cases] >>
+ rpt strip_tac >>
+
+ PairCases_on ‘BDD’ >>
+ rename1 ‘(root,edges,labels)’ >>
+
+ rgs[] >>
+
+ Cases_on ‘ALOOKUP edges n’ >> gvs[] >| [
+    gvs[BDD_WF_def, is_lookup_leaf_def]
+    ,
+    PairCases_on ‘x’ >> gvs[] >>
+    subgoal ‘∃pred x'.ALOOKUP labels n = SOME (non_termn (SOME x',pred))’ >-
+     (
+     gvs[BDD_WF_def, is_lookup_non_leaf_def, is_lookup_defined_def] >>
+     last_x_assum (strip_assume_tac o (Q.SPECL [‘n’])) >>
+     gvs[]
+     ) >>
+    gvs[] >>
+
+    subgoal ‘∃b . ALOOKUP mv x' = SOME b’ >-
+     (
+     gvs[mv_dom_bdd_def, is_lookup_defined_def]
+     ) >>
+
+    METIS_TAC[BDD_pred_sem_exsists_inter]
+  ]
+QED
+
+
+
+
+(*
+
+ (**********)     
+
+              
+                                 
+Theorem new_layer_correct:
+  ∀ BDD BDD'' vars_consumed h c c' mv.
+    correct_sem BDD ∧
+    BDD_WF BDD ∧
+    BDD_ordered BDD vars_consumed ∧
+    mv_dom_bdd mv BDD  ∧
+    consumed_dom_bdd vars_consumed BDD ∧
+    body_of_mk BDD h c = SOME (BDD'',c')
+    ==>
+    correct_sem BDD''
+Proof
+
+  namedCases ["r edges labels"] >>
+  namedCases ["r'' edges'' labels''"] >>
+
+  gvs[correct_sem_def] >>            
+  Induct_on ‘BDD_pred_sem’ >>
+  rpt strip_tac >> gvs[] >|[
+
+    gvs[get_prop_def] >>
+    Cases_on ‘p’ >>gvs[] >>
+    Cases_on ‘p'’ >> gvs[from_pred_to_bool_def, apply_Sem_rule_def, Sem_rule_def]
+
+    ,
+
+    ‘r''=r’ by (gvs[body_of_mk_def] >> gvs[AllCaseEqs()]) >> gvs[] >>       
+
+    RES_TAC >>
+
+    
+
+            
+    ‘apply_Sem_rule (get_prop labels' n') mv = apply_Sem_rule (get_prop labels' n) mv’ 
+
+            
+    simp[Once get_prop_def] >>
+    simp[apply_Sem_rule_def] >>
+    gvs[]
+
+    gvs[Once BDD_pred_sem_cases] >|[
+
+        ‘’
+
+   cheat
+
+
+      ]
+
+  ]
+
+
+  (*      
+  rpt strip_tac >>
+  PairCases_on ‘BDD’ >>
+  rename1 ‘(r,edges,labels)’ >>
+
+  PairCases_on ‘BDD''’ >>
+  rename1 ‘(r'',edges'',labels'')’ >>
+
+  ‘r''=r’ by (gvs[body_of_mk_def] >> gvs[AllCaseEqs()]) >> gvs[] >>       
+          
+  simp[correct_sem_def] >>
+  rpt strip_tac >>
+
+  gvs[Once BDD_pred_sem_cases] >| [
+    gvs[get_prop_def] >>
+    Cases_on ‘p’ >>gvs[] >>
+    Cases_on ‘p'’ >> gvs[from_pred_to_bool_def, apply_Sem_rule_def, Sem_rule_def]
+    ,
+    gvs[get_prop_def] >>
+    gvs[apply_Sem_rule_def]
+    
+    (* this is too easy, check with the boss *)
+  ]
+*)
+QED
+        
+
+
+        
+
+
+
+
+
+
+        
+Theorem lookup_labels_in_updt:
+∀ labels n x p h.
+ALOOKUP labels n = SOME (non_termn (SOME x,p)) ⇒
+ALOOKUP (non_term_leaf_updt labels h) n = SOME (non_termn (SOME x,p))
+Proof
+Induct >>
+rpt strip_tac >>
+simp[non_term_leaf_updt_def] >>
+PairCases_on ‘h’ >> gvs[ALOOKUP_def] >>
+gvs[AllCaseEqs()] >>
+Cases_on ‘h1’ >> gvs[] >>
+last_x_assum (strip_assume_tac o (Q.SPECL [‘n’, ‘x’, ‘p’, ‘h'’])) >>
+gvs[non_term_leaf_updt_def] >>
+Cases_on ‘p'’ >> gvs[] >>
+Cases_on ‘q’ >> gvs[]
+QED
+    
+
+
+
+
+        
+Theorem lookup_labels_in_updt_none:
+∀ labels n x p h.
+ALOOKUP labels n = SOME (non_termn (NONE,p)) ⇒
+ALOOKUP (non_term_leaf_updt labels h) n = SOME (non_termn (SOME h,p))
+Proof
+Induct >>
+rpt strip_tac >>
+gvs[ALOOKUP_def] >>
+
+gvs[Once non_term_leaf_updt_cons] >>
+rgs[ALOOKUP_APPEND]>>
+gvs[AllCaseEqs()] >>
+
+PairCases_on ‘h’ >> 
+gvs[AllCaseEqs()] >>
+simp[non_term_leaf_updt_def] >>
+
+
+Cases_on ‘h1’ >> gvs[] >>
+Cases_on ‘p'’ >> gvs[] >>
+Cases_on ‘q’ >> gvs[]
+QED
+    
+
+
+
+        
+Theorem WF_imp_non_leaf_lbl:
+∀ r edges labels n n' n'' h.      
+BDD_WF (r,edges,labels) ∧
+ALOOKUP edges n = SOME (n',n'') ⇒
+∃ x p . ALOOKUP labels n = SOME (non_termn (SOME x,p))
+Proof
+gvs[BDD_WF_def] >>
+rpt strip_tac >>
+last_x_assum (strip_assume_tac o (Q.SPECL [‘n’])) >> gvs[is_lookup_defined_def, is_lookup_non_leaf_def] 
+QED
+
+
+Theorem wf_lookup_if_edges_label:    
+∀ r edges labels n n' n'' h.      
+BDD_WF (r,edges,labels) ∧
+ALOOKUP edges n = SOME (n',n'') ⇒
+∃ x p . ALOOKUP (non_term_leaf_updt labels h) n = SOME (non_termn (SOME x,p))
+Proof
+rpt strip_tac >>                                                                  
+IMP_RES_TAC WF_imp_non_leaf_lbl >>
+IMP_RES_TAC lookup_labels_in_updt >>                      
+gvs[]
+QED
+
+
+
+
+
+
+
+
+
+
+
+
+Theorem lookup_new_edges_simp_exists:
+∀ simp_leaves' new_edges nn n c.
+  ALOOKUP new_edges n = SOME nn ∧
+  mk_new_edges simp_leaves' c = new_edges ⇒
+∃ sll . ALOOKUP simp_leaves' n = SOME sll
+Proof
+Induct >> 
+rgs[mk_new_edges_def]>>         
+rpt strip_tac >>
+PairCases_on ‘h’ >>
+rgs[mk_new_edges_def] >>
+rgs[AllCaseEqs()] >>
+RES_TAC >> gvs[]
+QED
+
+
+Theorem lookup_simp_leaves_determine_exists:
+∀ simp_leaves simp_leaves' n sll.        
+ALOOKUP simp_leaves' n = SOME sll ∧        
+determine_termn_list simp_leaves = simp_leaves' ⇒
+∃ sll' . ALOOKUP simp_leaves n = SOME sll'
+Proof
+Induct >> 
+rgs[determine_termn_list_def]>>         
+rpt strip_tac >>
+PairCases_on ‘h’ >>
+rgs[determine_termn_def] >>
+rgs[AllCaseEqs()] >>
+RES_TAC >> gvs[]
+QED
+
+
+
+Theorem  lookup_simp_pred_leaves_sub_exists:      
+∀ leaves_sub simp_leaves n sll.
+ALOOKUP simp_leaves n = SOME sll ∧        
+simp_pred_list leaves_sub = simp_leaves ⇒
+∃ sll' . ALOOKUP leaves_sub n = SOME sll'
+Proof
+Induct >> 
+rgs[simp_pred_list_def]>>         
+rpt strip_tac >>
+PairCases_on ‘h’ >>
+rgs[AllCaseEqs()]
+QED
+
+
+Theorem lookup_leaves_sub_pred_exists:
+∀ ntl  leaves_sub sll n h.       
+ALOOKUP leaves_sub n = SOME sll ∧
+leaves_pred_sub ntl h = leaves_sub ⇒
+∃ p . ALOOKUP ntl n = SOME p
+Proof
+Induct >> 
+rgs[leaves_pred_sub_def]>>         
+rpt strip_tac >>
+PairCases_on ‘h’ >>
+rgs[AllCaseEqs()] >>
+RES_TAC >> gvs[]
+QED                
+
+
+
+Theorem extract_nontermn_not_inner_node:                   
+∀ leaves ntl n .                            
+extract_nontermn leaves = SOME ntl ⇒
+∃ x p' . ALOOKUP leaves n ≠ SOME (non_termn (SOME x,p'))
+Proof
+Induct >-
+rgs[extract_nontermn_def]>>         
+rpt strip_tac >>
+PairCases_on ‘h’ >>
+gvs[]>>
+Cases_on ‘h0=n’ >> gvs[] >> rgs[extract_nontermn_def] >>                   
+Cases_on ‘h1’ >> rgs[AllCaseEqs()]
+QED
+
+
+
+        
+Theorem lookup_ntl_updt_none:
+∀ labels h n .
+ALOOKUP (non_term_leaf_updt labels h) n = NONE ⇒
+ALOOKUP labels n = NONE
+Proof
+Induct >- gvs[non_term_leaf_updt_def] >>                        
+rpt strip_tac >>
+gvs[Once non_term_leaf_updt_cons] >>
+gvs[] >>
+
+PairCases_on ‘h’>>
+rgs[AllCaseEqs()] >>
+                        
+gvs[ALOOKUP_APPEND] >>
+rgs[AllCaseEqs()] >>
+
+RES_TAC >> 
+gvs[non_term_leaf_updt_def] >>          
+Cases_on ‘h1’ >> gvs[] >>
+Cases_on ‘p’ >> gvs[] >>
+Cases_on ‘q’ >> gvs[]
+QED
+
+
+        
+Theorem mk_body_map1:
+∀ leaves labels leaves_labels .        
+getLabels labels leaves = SOME leaves_labels ⇒
+(leaves = MAP FST  leaves_labels)
+Proof
+  Induct >>
+  rpt strip_tac >>
+  gvs[getLabels_def] >>
+  REPEAT (BasicProvers.FULL_CASE_TAC >> gvs[]) >>
+  RES_TAC 
+QED
+
+
+Theorem mk_body_map2:
+  ∀ ntl leaves_sub h.
+    leaves_pred_sub ntl h = leaves_sub ⇒
+    MAP FST ntl = MAP FST leaves_sub 
+Proof
+  Induct >>
+  gvs[leaves_pred_sub_def] >>
+  rpt strip_tac >>
+  PairCases_on ‘h’ >> gvs[] 
+QED
+
+        
+Theorem mk_body_map3:
+  ∀ leaves_sub simp_leaves h.
+    simp_pred_list leaves_sub = simp_leaves ⇒
+    MAP FST leaves_sub = MAP FST simp_leaves 
+Proof
+  Induct >>
+  gvs[simp_pred_list_def] >>
+  rpt strip_tac >>
+  PairCases_on ‘h’ >> gvs[] 
+QED
+
+
+Theorem mk_body_map4:
+  ∀ leaves_simp leaves_simp' h.
+    determine_termn_list leaves_simp = leaves_simp' ⇒
+    MAP FST leaves_simp = MAP FST leaves_simp' 
+Proof
+  Induct >>
+  gvs[determine_termn_list_def] >>
+  rpt strip_tac >>
+  PairCases_on ‘h’ >> gvs[] 
+QED
+
+        
+Theorem mk_body_map5:
+  ∀ leaves_simp' new_edges c.
+    mk_new_edges leaves_simp' c = new_edges ⇒
+    MAP FST leaves_simp' = MAP FST new_edges
+Proof
+  Induct >>
+  gvs[mk_new_edges_def] >>
+  rpt strip_tac >>
+  PairCases_on ‘h’ >> gvs[mk_new_edges_def] 
+QED
+
+
+
+Theorem mk_body_map6:
+  ∀ labels updated_labels x.
+    non_term_leaf_updt labels x = updated_labels ⇒
+    MAP FST labels = MAP FST updated_labels
+Proof
+  Induct >>
+  gvs[non_term_leaf_updt_def] >>
+  rpt strip_tac >>
+  PairCases_on ‘h’ >>
+  gvs[AllCaseEqs()] >>                      
+  Cases_on ‘h1’ >> gvs[] >>
+  Cases_on ‘p’ >> gvs[] >>
+  Cases_on ‘q’ >> gvs[]
+QED
+
+
+
+
+
+        
+        
+        
+Theorem extract_nonterm_mem_neg:        
+∀ leaves_labels ntl h.
+¬MEM h (MAP FST leaves_labels) ∧
+extract_nontermn leaves_labels = SOME ntl ⇒
+¬MEM h (MAP FST ntl)
+Proof
+  Induct >>
+  rpt strip_tac >>
+  gvs[extract_nontermn_def] >>
+  PairCases_on ‘h’ >> gvs[] >>
+  gvs[extract_nontermn_def] >>
+  gvs[AllCaseEqs()]                      
+QED
+
+
+        
+  
+
+Theorem all_distinct_leaves:
+∀ edges r leaves .        
+ALL_DISTINCT (MAP FST edges) ∧
+getLeaves edges r = leaves ⇒
+ALL_DISTINCT leaves
+Proof
+Induct >>
+gvs[getLeaves_def] >>
+rpt strip_tac >>
+gvs[AllCaseEqs()] >>
+PairCases_on ‘h’ >>
+gvs[get_leaves_list_def]
+QED
+
+
+
+Theorem all_distinct_leaves_labels:
+∀ leaves labels leaves_labels .        
+ALL_DISTINCT leaves ∧
+getLabels labels leaves = SOME leaves_labels ⇒
+ALL_DISTINCT (MAP FST leaves_labels)
+Proof
+rpt strip_tac >>
+imp_res_tac mk_body_map1 >>
+gvs[]
+QED
+
+        
+ 
+        
+Theorem all_distinct_ntl:
+  ∀ leaves_labels ntl .
+  ALL_DISTINCT (MAP FST leaves_labels) ∧
+  extract_nontermn leaves_labels = SOME ntl ⇒
+  ALL_DISTINCT (MAP FST ntl)                  
+Proof
+  Induct >>
+  rpt strip_tac >>
+  gvs[extract_nontermn_def] >>
+  PairCases_on ‘h’ >> gvs[] >>
+  gvs[extract_nontermn_def] >>
+  gvs[AllCaseEqs()] >>
+  imp_res_tac extract_nonterm_mem_neg
+QED   
+
+
+
+
+
+Theorem all_distinct_sub:
+  ∀ ntl leaves_sub h.
+    ALL_DISTINCT (MAP FST ntl) ∧
+    leaves_pred_sub ntl h = leaves_sub ⇒
+    ALL_DISTINCT (MAP FST leaves_sub) 
+Proof
+  rpt strip_tac >>
+  imp_res_tac mk_body_map2 >>
+  gvs[] 
+QED
+
+
+        
+Theorem all_distinct_simp:
+  ∀ simp_leaves leaves_sub h.
+    ALL_DISTINCT (MAP FST leaves_sub) ∧
+    simp_pred_list leaves_sub = simp_leaves ⇒
+         ALL_DISTINCT (MAP FST simp_leaves)               
+Proof
+  rpt strip_tac >>
+  imp_res_tac mk_body_map3 >>
+  gvs[]  
+QED
+
+
+
+Theorem all_distinct_determine:
+  ∀ simp_leaves simp_leaves' h.
+    ALL_DISTINCT (MAP FST simp_leaves) ∧
+    determine_termn_list simp_leaves = simp_leaves' ⇒
+         ALL_DISTINCT (MAP FST simp_leaves')               
+Proof
+  rpt strip_tac >>
+  imp_res_tac mk_body_map4 >>
+  gvs[]  
+QED
+
+
+
+        
+Theorem all_distinct_mk_edges:
+  ∀ simp_leaves' new_edges c.
+    ALL_DISTINCT (MAP FST simp_leaves') ∧
+    mk_new_edges simp_leaves' c = new_edges ⇒
+    ALL_DISTINCT (MAP FST new_edges)               
+Proof
+  rpt strip_tac >>
+  imp_res_tac mk_body_map5 >>
+  gvs[]  
+QED
+
+
+
+        
+Theorem all_distinct_non_term_leaf_updt:        
+∀ labels updated_labels h.
+  ALL_DISTINCT (MAP FST labels) ∧
+  non_term_leaf_updt labels h = updated_labels ⇒
+  ALL_DISTINCT (MAP FST updated_labels)
+Proof
+  rpt strip_tac >>
+  imp_res_tac mk_body_map6 >>
+  gvs[]
+QED
+
+
+
+
+
+Triviality mk_new_label_idx_mem:
+  ∀ simp_leaves n c.
+    n>0 ⇒
+    ¬MEM c (MAP FST (mk_new_labels simp_leaves (c + n))) 
+Proof
+Induct >>
+gvs[mk_new_labels_def] >>
+rpt gen_tac >>
+PairCases_on ‘h’ >>
+simp[mk_new_labels_def]
+QED
+
+
+
+       
+
+Theorem all_distinct_mk_labels:      
+  ∀ simp_leaves' new_labels c.
+    ALL_DISTINCT (MAP FST simp_leaves') ∧
+    mk_new_labels simp_leaves' c = new_labels ⇒
+    ALL_DISTINCT (MAP FST new_labels)               
+Proof
+  Induct >>
+  rgs[Once mk_new_labels_def] >>
+  rpt strip_tac >>
+  rgs[Once mk_new_labels_def] >>
+  PairCases_on ‘h’ >>
+  simp[Once mk_new_labels_def] >>
+  gvs[mk_new_label_idx_mem] >>
+  assume_tac mk_new_label_idx_mem >>
+  first_x_assum (strip_assume_tac o (Q.SPECL [‘simp_leaves'’,‘1’,‘c+1’])) >>
+  gvs[]           
+QED
+
+
+
+
+
+
+ 
+Theorem get_leaves_list_domain:
+  ∀ edges leaves n.     
+    MEM n (MAP FST edges) ∧
+    get_leaves_list edges = leaves
+    ⇒
+    ~ MEM n leaves
+Proof
+  Induct >>
+  rpt strip_tac >- gvs[get_leaves_list_def] >>
+  PairCases_on ‘h’ >>
+  rgs[] >>
+  res_tac >>
+  rgs[Once get_leaves_list_def] >>
+  gvs[get_leaves_list_def] >>
+  REPEAT (BasicProvers.FULL_CASE_TAC >> rgs[]) >>
+  rgs[MEM_FILTER]
+QED
+
+
+Triviality getLeaves_list_eq:      
+∀ l h r .
+getLeaves (h::l) r = get_leaves_list (h::l)
+Proof                                        
+gvs[getLeaves_def, get_leaves_list_def]
+QED
+
+
+
+
+        
+Theorem leaves_are_not_parents:         
+∀ edges leaves n r.     
+  MEM n (MAP FST edges) ∧
+  getLeaves edges r = leaves ⇒
+  ~ MEM n leaves
+Proof
+  Cases_on ‘edges’ >>
+  rpt strip_tac >-
+   gvs[getLeaves_def] >>
+  imp_res_tac get_leaves_list_domain >>
+  rgs[Once getLeaves_list_eq]          
+QED
+
+
+
+
+                     
+      
+
+        
+Theorem WFness_translation:
+  ∀ vars vars_consumed BDD BDD' c.
+    BDD_WF BDD ⇒
+    (SOME BDD' = mk_BDDPred BDD vars_consumed vars c) ⇒
+    BDD_WF BDD' 
+Proof
+  Induct >| [
+    rpt strip_tac >>
+    PairCases_on ‘BDD’ >> gvs[] >>
+    gvs[mk_BDDPred_def]
+    ,
+    rpt strip_tac >>
+
+    PairCases_on ‘BDD’ >>
+    rename1 ‘(r,edges,labels)’ >>
+
+    PairCases_on ‘BDD'’ >>
+    rename1 ‘(r',edges',labels')’ >>
+
+    gvs[mk_BDDPred_def] >>
+    gvs[body_of_mk_def] >>
+    REPEAT (BasicProvers.FULL_CASE_TAC >> gvs[]) >>
+
+    
+    ‘∃ leaves_sub . leaves_pred_sub x' h = leaves_sub’ by gvs[] >>
+    ‘∃ simp_leaves . simp_pred_list leaves_sub = simp_leaves’ by gvs[] >>
+    ‘∃ simp_leaves' . determine_termn_list simp_leaves = simp_leaves'’ by gvs[] >>
+    ‘∃ new_edges . mk_new_edges simp_leaves' c = new_edges’ by gvs[] >>
+    ‘∃ new_labels . mk_new_labels simp_leaves' c = new_labels’ by gvs[] >>
+    
+    rgs[] >>
+
+
+    subgoal ‘ALL_DISTINCT (MAP FST edges ⧺ MAP FST new_edges)’ >- (
+            
+      ‘ALL_DISTINCT (MAP FST edges)’ by rgs[Once BDD_WF_def] >>
+      ‘∃ leaves. getLeaves edges r = leaves’ by gvs[] >>
+
+      imp_res_tac all_distinct_leaves >>
+      ‘ALL_DISTINCT (MAP FST x)’ by (imp_res_tac all_distinct_leaves_labels >> gvs[]) >>
+      imp_res_tac all_distinct_ntl >>       
+      imp_res_tac all_distinct_sub >>
+      imp_res_tac all_distinct_simp >>
+      ‘ALL_DISTINCT (MAP FST simp_leaves')’ by (imp_res_tac all_distinct_determine >> gvs[]) >>        
+      ‘ALL_DISTINCT (MAP FST new_edges)’ by (imp_res_tac all_distinct_mk_edges >> gvs[]) >>
+                  
+      simp[ALL_DISTINCT_APPEND]>>
+      strip_tac >> strip_tac >>
+      imp_res_tac leaves_are_not_parents>>
+
+      imp_res_tac mk_body_map1 >>
+      imp_res_tac mk_body_map2 >>
+      imp_res_tac mk_body_map3 >>
+      imp_res_tac mk_body_map4 >>
+      imp_res_tac mk_body_map5 >>
+      rgs[] >>
+
+      imp_res_tac extract_nonterm_mem_neg >>   
+      gvs[ALOOKUP_NONE]
+      ) >>
+
+
+
+
+
+    subgoal ‘ALL_DISTINCT (MAP FST (non_term_leaf_updt labels h) ⧺ MAP FST new_labels)’ >-(
+
+      ‘ALL_DISTINCT (MAP FST labels)’ by rgs[Once BDD_WF_def] >>
+      ‘ALL_DISTINCT (MAP FST (non_term_leaf_updt labels h))’ by (imp_res_tac all_distinct_non_term_leaf_updt >> gvs[]) >>
+
+
+
+
+      (* same as before *)
+      ‘ALL_DISTINCT (MAP FST edges)’ by rgs[Once BDD_WF_def] >>
+      ‘∃ leaves. getLeaves edges r = leaves’ by gvs[] >>
+
+      imp_res_tac all_distinct_leaves >>
+      ‘ALL_DISTINCT (MAP FST x)’ by (imp_res_tac all_distinct_leaves_labels >> gvs[]) >>
+      imp_res_tac all_distinct_ntl >>       
+      imp_res_tac all_distinct_sub >>
+      imp_res_tac all_distinct_simp >>
+      ‘ALL_DISTINCT (MAP FST simp_leaves')’ by (imp_res_tac all_distinct_determine >> gvs[]) >>        
+      ‘ALL_DISTINCT (MAP FST new_edges)’ by (imp_res_tac all_distinct_mk_edges >> gvs[]) >>
+      (*end*)
+                    
+      ‘ALL_DISTINCT (MAP FST new_labels)’ by (imp_res_tac all_distinct_mk_labels >> gvs[]) >>        
+      simp[ALL_DISTINCT_APPEND]>>
+
+      strip_tac >> strip_tac >>
+      imp_res_tac leaves_are_not_parents>>
+      (*if in labels changed, then in labels, then from efness in *)
+
+
+
+      imp_res_tac mk_body_map1 >>
+      imp_res_tac mk_body_map2 >>
+      imp_res_tac mk_body_map3 >>
+      imp_res_tac mk_body_map4 >>
+      imp_res_tac mk_body_map5 >>
+      imp_res_tac mk_body_map6 >>
+
+      rgs[] >>
+
+      imp_res_tac extract_nonterm_mem_neg >>   
+      rgs[ALOOKUP_NONE] >>
+
+      (* here ? *)   
+
+
+      ‘MEM e (MAP FST (labels))’ by cheat >>
+      ‘MEM e (MAP FST (edges))’ by cheat >>
+
+      gvs[ALOOKUP_NONE] >>
+      ‘¬MEM e (MAP FST x)’ by res_tac >>
+      ‘¬MEM e (MAP FST new_edges)’ by res_tac >>
+      cheat
+      ) >>
+
+
+
+
+
+
+
+
+      
+          
+    subgoal ‘BDD_WF (r,edges ⧺ new_edges,non_term_leaf_updt labels h ⧺ new_labels)’ >-  (
+      simp[BDD_WF_def] >> CONJ_TAC >> rpt strip_tac  >| [
+                       
+          (* internal nodes *)
+             
+          rgs[is_lookup_defined_def, is_lookup_non_leaf_def] >>
+          rgs[ALOOKUP_APPEND] >>
+          
+          Cases_on ‘ALOOKUP edges n’ >> rgs[] >|[
+                   
+            (* if not in old edges, and in the new edges , ALOOKUP edges n = NONE*)
+            
+            Cases_on ‘ALOOKUP (non_term_leaf_updt labels h) n’ >>
+            REPEAT (BasicProvers.FULL_CASE_TAC >> rgs[]) >|[
+              (* this is false *)
+              rgs[BDD_WF_def] >>
+              rgs[is_lookup_leaf_def] >>
+              imp_res_tac lookup_ntl_updt_none >>
+              gvs[]
+              ,
+              (* this was a leaf in edges, and then it became a parent in BDD''*)
+              (* Cases_on ‘x''''’ >> rgs[] >>*)
+              
+              rgs[BDD_WF_def] >|[
+                  
+                  rgs[is_lookup_leaf_def]>>
+                  imp_res_tac lookup_labels_in_updt_none >>
+                  ‘x'⁴' = non_termn (SOME h,p)’ by gvs[] >>
+                  rgs[is_lookup_non_leaf_def, is_lookup_defined_def] >>
+                  ‘ALOOKUP edges n = NONE’ by res_tac >>
+                  rgs[ALL_DISTINCT_APPEND]>>
+                  cheat
+                  ,
+                  cheat
+                  ,
+                  cheat
+                  
+                ]                                   
+            ]                                
+            ,
+          (* if not in new edges, and in old edges i.e. ALOOKUP edges n = SOME x'³'*)
+          
+          Cases_on ‘ALOOKUP (non_term_leaf_updt labels h) n’ >> rgs[] >|[
+                rgs[BDD_WF_def] >>
+                rgs[is_lookup_leaf_def] >>
+                imp_res_tac lookup_ntl_updt_none >>
+                rgs[is_lookup_defined_def, is_lookup_non_leaf_def] >>
+                res_tac >>
+                gvs[]
+                ,
+                imp_res_tac wf_lookup_if_edges_label >>
+                PairCases_on ‘x'''’ >>
+                ‘∃x p. ALOOKUP (non_term_leaf_updt labels h) n =
+                       SOME (non_termn (SOME x,p))’ by (res_tac >> gvs[]) >>
+                gvs[]
+              ]
+          ] 
+                                                
+          ,
+                
+          (* leafs*)
+
+
+          rgs[is_lookup_leaf_def] >>
+          rgs[ALOOKUP_APPEND] >>
+
+          Cases_on ‘ALOOKUP edges n’ >> rgs[] >|[
+              
+
+
+            ]
+          
+          
+
+                              
+          cheat
+        ]                                           
+      ) >>
+    RES_TAC
+QED
+
+     
+
+(* this proof requires WFness and ordered for intermidiate steps to be proven*)        
+
+Theorem correct_sem_translation:
+  ∀ vars vars_consumed BDD BDD' c.
+    BDD_ordered BDD vars_consumed ∧
+    correct_sem BDD ⇒
+    (SOME BDD' = mk_BDDPred BDD vars_consumed vars c) ⇒
+    correct_sem BDD' 
+Proof
+  Induct >| [
+    rpt strip_tac >>
+    gvs[mk_BDDPred_def]
+    ,
+    rpt strip_tac >>
+
+    gvs[mk_BDDPred_def] >>
+    gvs[AllCaseEqs()] >>
+    ‘correct_sem BDD''’ by cheat >>
+    ‘BDD_ordered  BDD'' (h::vars_consumed)’ by cheat >>
+    RES_TAC >> METIS_TAC[]
+  ]
+QED
+
+
+
+
+(*****************************)
+(*********   MERGE    ********)
+(*****************************)
+
+
+Definition mergable_def:        
+mergable ((r,edges,labels):BDD)  n n' = 
+(ALOOKUP edges n = ALOOKUP edges n' ∧
+ ALOOKUP labels n = ALOOKUP labels n' ∧ ALOOKUP labels n'  ≠ NONE )
+End
+
+
+
+
+        
+Definition merge_def:
+  merge ((r,edges,labels):BDD) n n' =
+   MAP (\(a,b,c). ( a, if (b=n' ∧ c=n') then (n,n)
+                 else if (b=n') then (n,c)
+                 else if (c=n') then (b,n)
+                     else (b,c))) edges 
+End
+
+
+EVAL “merge (1,[(1,2,3);(2,4,5);(3,4,5)],[]) 2 3”
+
+
+
+
+
+
+        
+∀ edges n'' n' n r labels.
+n'' ≠ n' ∧       
+MEM n'' (nodes_list edges) ⇒
+MEM n'' (nodes_list (point_parents (r,edges,labels) n n'))       
+
+
+
+
+
+
+
+
+
+                
+(*Lemma 3*)
+
+∀ labels vars_consumed n'' r edges n' n mv.
+BDD_ordered (r,edges,labels) vars_consumed ∧
+mergable (r,edges,labels) n n' ⇒
+Sem_BDDpred (r,edges,labels) mv n'' = Sem_BDDpred (r,merge (r,edges,labels) n n',labels) mv n''
+
+
+ NTAC 3 strip_tac >>
+  measureInduct_on `get_string_in_label labels  vars_consumed n''` >>
+                                                                   
+rpt strip_tac >>
+simp[Sem_BDDpred_def]>>
+simp[Once Sem_BDDpred_fun_def] >|[
+    Cases_on ‘¬MEM n'' (nodes_list edges)’ >> gvs[] >|[
+      ‘~ MEM n'' (nodes_list (point_parents (r,edges,labels) n n'))’ by cheat >>
+      simp[Once Sem_BDDpred_fun_def]
+      ,
+      Cases_on ‘ALOOKUP edges n''’ >> gvs[] >|[
+          Cases_on ‘ALOOKUP labels n''’ >> gvs[] >|[
+            cheat
+            ,
+            cheat
+           (* Cases_on ‘x’ >> gvs[] >|[
+                (* if termin*)
+                ‘p = True ∨ p = False’ by cheat >> gvs[] >>
+                simp[Once EQ_SYM_EQ, Once Sem_BDDpred_fun_def] >>
+                Cases_on ‘ALOOKUP (point_parents (r,edges,labels) n n') n''’ >> gvs[] >>
+                ‘n'' ≠ n'’ by cheat >> (* again incorrect theorem *)
+                cheat
+                Cases_on ‘x’ >> gvs[] >>
+                cheat
+                ,
+                Cases_on ‘p’ >> gvs[] >>
+
+                simp[Once EQ_SYM_EQ, Once Sem_BDDpred_fun_def] >>
+                ‘MEM n'' (nodes_list (point_parents (r,edges,labels) n n'))’ by cheat >> gvs[] >>
+                ‘ALOOKUP (point_parents (r,edges,labels) n n') n'' = NONE’ by cheat >> gvs[]
+                Cases
+              ]                                      
+                                    
+          ]*)
+        ]
+          ,
+
+          PairCases_on ‘x’ >> gvs[] >>
+          Cases_on ‘ALOOKUP labels n''’ >> gvs[] >|[
+              cheat
+              ,
+              Cases_on ‘x’ >> gvs[] >| [
+                  cheat
+                  ,
+                  Cases_on ‘p’ >> gvs[] >> Cases_on ‘q’ >> gvs[] >|[
+                      cheat
+                      ,
+                      Cases_on ‘ALOOKUP mv x’ >> gvs[] >| [
+                          cheat
+                          ,
+                          Cases_on ‘x'’ >> gvs[] >| [
+                              simp[Once EQ_SYM_EQ, Once Sem_BDDpred_fun_def] >>
+                              Cases_on ‘¬MEM n'' (nodes_list (point_parents (r,edges,labels) n n'))’ >> gvs[]  >|[
+                                (* if we do not find it, then it must have been merged, thus, n'' = n' *)
+                                   ‘n'' = n'’ by cheat >>
+                                   gvs[] >>
+                                      (* this is an incorrect theorem as the merged node actually disappears..
+                                      thus in the onld one it had semantics, and in the new one it does not*)
+                                   cheat >> (*problem *)
+                                   ,
+                                   Cases_on ‘ALOOKUP (point_parents (r,edges,labels) n n') n''’ >> gvs[]  >| [
+                                       gvs[ALOOKUP_MEM]
+                                   cheat    
+                                   ,
+                                   Cases_on ‘x'’ >> gvs[] >>
+                                   (* we check if these are parents or not of merged, they are parents if their
+                                      indexes changed in teh graph*)
+                                   Cases_on ‘ALOOKUP (point_parents (r,edges,labels) n n') n'' =
+                                             ALOOKUP edges n''’ >> gvs[] >| [
+                                       (* not a changed parent *)
+                                       
+                                       subgoal ‘get_string_in_label labels vars_consumed r'' <
+                                                get_string_in_label labels vars_consumed n''’ >-(
+                                       rgs[Once BDD_ordered_def] >>
+                                       first_x_assum (strip_assume_tac o (Q.SPECL [‘n''’,‘q’,‘r''’,‘x’,‘x'’,‘’])) >>
+                                       gvs[get_string_in_label_def] >>
+                                       Cases_on ‘ALOOKUP labels r''’ >> gvs[]
+
+                                                
+                                       )
+
+                                          
+                                       ‘get_string_in_label labels vars_consumed r'' <
+                                        get_string_in_label labels vars_consumed n''’ by cheat >>
+
+                                       first_x_assum (strip_assume_tac o (Q.SPECL [‘r''’])) >>
+                                       gvs[] >>
+                                        
+                                       first_x_assum (strip_assume_tac o (Q.SPECL [‘r’,
+                                                                                   ‘edges’,
+                                                                                   ‘n'’, ‘n’, ‘mv’])) >>
+                                        
+                                       gvs[] >>
+                                       rgs[Sem_BDDpred_def] >>
+                                       cheat
+                                       ,
+                                       (* this means that teh parent has changed and
+                                       rerouted to new choldren*)
+
+
+                                       Cases_on ‘q=x0’ >> gvs[] >|[
+                                            ‘x1=n'’ by cheat >> gvs[] >>                    
+                                            ‘r''=n’ by cheat >> gvs[] >>
+                                            gvs[mergable_def]
+
+                                        
+                                     ]
+                                           
+
+                                     ]
+                                   
+                              ]
+                            ]
+
+                        ]
+
+                    ] 
+                  
+                ]
+
+            ]                                         
+          
+                                                   
+        ]
+                                              
+
+                                              
+                                              
+                                              
+    ]
+
+
+
+
+
+
+  ]
+
+
+
+
+
+
+
+
+
+
 
 
                                                                    
 
 
-Definition nodes_set_def:
-  nodes_set (edges:'a edges) =        
-  set (MAP FST edges) ∪ set (MAP (SND o SND) edges) ∪ set (MAP (FST o SND) edges)
-End
-
-
-
-Definition mk_distinct_def:
-  mk_distinct [] = [] ∧
-  mk_distinct (h::l) = if (MEM h l) then
-                         mk_distinct l
-                       else
-                         h::(mk_distinct l)       
-End
-
-
-Theorem mk_distinct_nub_eq:
-  ∀ l . mk_distinct l = nub l
-Proof
-  Induct_on ‘l’ >>
-  gvs[mk_distinct_def,nub_def]
-QED
-        
-
-
-Theorem mk_distinct_mem:
-  ∀ l r. MEM r l = MEM r (mk_distinct l)
-Proof
-  fs[mk_distinct_nub_eq]
-QED
-
-        
-        
-Definition nodes_list_def:
-  nodes_list (edges:'a edges) =        
-  let 
-    parents = MAP FST edges;
-    children_right = MAP (SND o SND) edges ;
-    children_left  = MAP (FST o SND) edges
-  in
-    mk_distinct(parents ++ children_right ++ children_left)
-End
-
-
-Triviality UNION_APPEND_tri:
-∀ l1 l2 l3. set l1 ∪ set l2 ∪ set l3 = set (l1 ++ l2 ++ l3 )
-Proof
-  gvs[Once UNION_APPEND]
-QED
-        
-
-Theorem nodes_set_list_length_eq:
-  ∀ edges . CARD (nodes_set edges) = LENGTH (nodes_list edges)
-Proof
-  gvs[nodes_list_def, nodes_set_def, mk_distinct_nub_eq] >>
-  strip_tac >>
-  assume_tac UNION_APPEND_tri  >>             
-  first_x_assum $ qspecl_then [‘MAP FST edges : 'a list’,
-                               ‘MAP (SND ∘ SND) edges  : 'a list’,
-                               ‘MAP (FST ∘ SND) edges : 'a list’] assume_tac >>
-  METIS_TAC[CARD_LIST_TO_SET_EQN]
-QED
-
-        
-
-Theorem nodes_set_list_mem_eq:
-∀ edges node. node ∈ nodes_set edges ⇔ MEM node (nodes_list edges) 
-Proof
-  fs[nodes_set_def,nodes_list_def, mk_distinct_def, MEM]>>
-  gvs[mk_distinct_nub_eq]
-QED
-
-
-Theorem nodes_set_eq1:
- ∀ edges.  nodes_set edges = set (nodes_list edges)     
-Proof
-  fs[nodes_set_def, nodes_list_def, LIST_TO_SET_DEF] >>
-  strip_tac >>
-  assume_tac UNION_APPEND_tri  >>             
-  first_x_assum $ qspecl_then [‘MAP FST edges : 'a list’,
-                               ‘MAP (SND ∘ SND) edges  : 'a list’,
-                               ‘MAP (FST ∘ SND) edges : 'a list’] assume_tac >>
-  gvs[mk_distinct_nub_eq] 
-QED
-
-(*
-The set of leaves are basically all nodes - (domain edges)
-*)
-Definition get_leaves_set_def:
-  get_leaves_set (edges:'a edges)  = 
-     (nodes_set edges) DIFF set (MAP FST edges)    
-End
-
-EVAL “ {(1:num);3} DIFF {(1:num);(2:num)}”;        
-
-
-Definition get_list_diff_def:
-  get_list_diff [] l2 = [] ∧
-  get_list_diff (h::l1) l2 =
-  if MEM h l2 then
-    get_list_diff l1 l2
-  else
-    h::(get_list_diff l1 l2)    
-End
-
-        
-Definition get_leaves_list_def:
-  get_leaves_list (edges:'a edges)  = 
-  let
-    all_nodes = nodes_list edges;
-    parents = MAP FST edges
-  in
-    get_list_diff all_nodes parents   
-End
-
-
-Triviality get_leaves_list_mem_imp:
-  ∀ l1 l2 l a.  l = get_list_diff l1 l2 ⇒
- (MEM a l ⇔ MEM a l1 ∧ ¬MEM a l2)
-Proof
-  Induct >> rpt strip_tac >>
-  fs[get_list_diff_def, MEM] >>      
-  gvs[AllCaseEqs()] >>
-  Cases_on ‘a=h’ >> gvs[]    
-QED
-
-
-Triviality get_list_diff_filter_eq:        
- ∀ l1 l2 .  get_list_diff l1 l2 = FILTER (λx. ¬MEM x l2) l1
-Proof
-  Induct >>
-  rpt strip_tac  >>
-  gvs[get_list_diff_def] >>
-  gvs[AllCaseEqs()]
-QED
 
 
         
-        
-Theorem get_leaves_set_list_mem_eq:
- ∀ edges node.  node ∈ (get_leaves_set edges) ⇔ MEM node (get_leaves_list edges)
+Theorem merge_correct:        
+  ∀ r edges labels vars_consumed n n'.
+        correct_sem (r,edges,labels) ∧
+        BDD_ordered (r,edges,labels) vars_consumed ∧           
+        mergable (r,edges,labels) n n'
+        ==>
+        correct_sem (r, point_parents (r,edges,labels) n n', labels)
 Proof
-  
-  simp_tac bool_ss [get_leaves_set_def]>>
-  gvs[list_to_set_diff]>>
-  gvs[get_leaves_list_def] >>
-  gvs[nodes_set_list_mem_eq] >>
-  gvs[get_leaves_list_mem_imp]
-QED
 
-
-
-Definition get_label_set_def:
-  get_label_set (labels: ('a,'b) labels) (nodes_set: 'a set) =
-  IMAGE (λx. (ALOOKUP labels x)) nodes_set    
-End
-
-
-
-Definition get_label_list_def:
-  get_label_list (labels: ('a,'b) labels) (nodes_list: 'a list) =
-  MAP (λx. (ALOOKUP labels x)) nodes_list   
-End
-
-
-
-Triviality get_label_set_list_eq1:
- ∀ labels edges . get_label_set labels (nodes_set edges) = set (get_label_list labels (nodes_list edges))
-Proof
-  gvs[get_label_set_def, get_label_list_def]>>
-  gvs[LIST_TO_SET_MAP] >>
+  rpt strip_tac >>   
+  simp[correct_sem_def] >>
   rpt strip_tac >>
-  gvs[nodes_set_eq1]
+  gvs[correct_sem_def] >>
+  first_x_assum (strip_assume_tac o (Q.SPECL [‘n''’,‘mv’])) >>
+  
+  ‘Sem_BDDpred (r,edges,labels) mv n'' = Sem_BDDpred (r,point_parents (r,edges,labels) n n',labels) mv n''’ by cheat >> gvs[]
 QED
-
-
-
-(*****************************************)
-
-
-     
-Definition mk_substitute_rule_def:
-  (mk_substitute_rule (c_b b') (x:'a) b = c_b b') ∧
-  (mk_substitute_rule (c_e (x':'a)) x b = if (x=x') then c_b b else c_e x') ∧
-  (mk_substitute_rule (c_and c c' ) x b =
-      (c_and (mk_substitute_rule c x b) (mk_substitute_rule c' x b ))) ∧
-  (mk_substitute_rule (c_or c c') x b =
-      (c_or (mk_substitute_rule c x b) (mk_substitute_rule c' x b ))) ∧
-  (mk_substitute_rule (c_neg c) x b=
-      (c_neg (mk_substitute_rule c x b)))
-End
-
-
-EVAL “mk_substitute_rule (c_and (c_e "x") (c_e "y")) "x" T”;        
-EVAL “mk_substitute_rule (c_and (c_or (c_e "x") (c_e "y")) (c_e "y")) "y" T”;        
-
-                     
-Definition mk_substitute_policy_list_def:
-  mk_substitute_policy_list (rules_list: 'a rule list) x b =
-       MAP (λ (c,a) . (mk_substitute_rule x b, a)) rules_list
-End
-
         
-
-       
-Definition mk_substitute_policy_set_def:
-   mk_substitute_policy_set (rules_set: 'a rule set ) x b =
-       IMAGE (λ (c,a) . (mk_substitute_rule x b, a)) rules_set
-End
-
-
-Triviality mk_substitute_policy_set_eq:
- ∀ (rule_list: 'a rule list) x b .  mk_substitute_policy_set (set rule_list) x b = set (mk_substitute_policy_list rule_list x b)
-Proof
-  gvs[mk_substitute_policy_set_def, mk_substitute_policy_list_def]>>
-  gvs[LIST_TO_SET_MAP] 
-QED
-
-
-
-(*************************************)
-Definition edges_acyclic_def:
-  edges_acyclic (edges:('a#'a#'a) set) =
-  let nr = IMAGE (λ(n,n',n''). (n,n'')) edges;
-      nl = IMAGE (λ(n,n',n''). (n,n')) edges
-  in
-     acyclic(nr ∪ nl)
-End
-(************************************)
+   *)     
+        
 
 
 val _ = export_theory ();
+
+    
